WIP: Update Minterop and RSP

IO.Behavior.fst
@@ -10,13 +10,13 @@ open IIO.Effect
 open MIO.Effect
 open MIIO.Effect
 
-type set_of_traces (a:Type) = events_trace * a -> Type0
+type set_of_traces (a:Type) = trace * a -> Type0
 
 val set_of_traces_ret : (#a:Type) -> a -> set_of_traces a
 let set_of_traces_ret x (es, x') = x == x' /\ es == []
 
 val set_of_traces_bind : (#a:Type) -> (#b:Type) -> set_of_traces a -> (a -> set_of_traces b) -> set_of_traces b
-let set_of_traces_bind p f (es, b) = exists (es1 es2 : events_trace) . exists a . es == (es1 @ es2) /\ p (es1, a) /\ f a (es2, b)
+let set_of_traces_bind p f (es, b) = exists (es1 es2 : trace) . exists a . es == (es1 @ es2) /\ p (es1, a) /\ f a (es2, b)
 
 val set_of_traces_map : (#a:Type) -> (#b:Type) -> (a -> b) -> set_of_traces a -> set_of_traces b
 let set_of_traces_map f p (es, b) = exists a . f a == b /\ p (es, a)
@@ -35,100 +35,101 @@ let rec behavior #a
   | Throw err -> fun t -> t == ([], Inr err)
   | Cont t -> begin
     match t with
-    | Call cmd args fnc -> (fun (t', r') -> 
-      (exists (res:resm cmd) t. (
-         FStar.WellFounded.axiom1 fnc res;
-         (behavior (fnc res) (t,r')) /\
-         t' == (convert_call_to_event cmd args res)::t)))
+    | Call cmd arg fnc -> (fun (t', r') -> 
+      (exists (r:io_resm cmd) t. (
+         FStar.WellFounded.axiom1 fnc r;
+         (behavior (fnc r) (t,r')) /\
+         t' == (convert_call_to_event cmd arg r)::t)))
   end
 
 let beh_shift_trace
   #a
   (cmd : io_cmds)
-  (argz : io_args cmd)
+  (arg : io_args cmd)
   (rez : io_resm cmd)
-  (fnc : io_resm cmd -> io a)
-  (t:events_trace)
+  (fnc : maybe (io_res cmd) -> io a)
+  (t:trace)
   (r:maybe a) :
   Lemma 
-    (requires (behavior (Cont (Call cmd argz fnc)) ((convert_call_to_event cmd argz rez :: t), r)))
+    (requires (behavior (Cont (Call cmd arg fnc)) ((convert_call_to_event cmd arg rez :: t), r)))
     (ensures (behavior (fnc rez) (t, r))) = 
   () 
 
 let beh_extend_trace 
   #a
   (cmd : io_cmds)
-  (argz : io_args cmd)
+  (arg : io_args cmd)
   (rez : io_resm cmd)
-  (fnc : io_resm cmd -> io a)
-  (t:events_trace)
+  (fnc : maybe (io_res cmd) -> io a)
+  (t:trace)
   (r:maybe a) :
   Lemma
     (requires (behavior (fnc rez) (t, r)))
-    (ensures (behavior (Cont (Call cmd argz fnc)) ((convert_call_to_event cmd argz rez) :: t, r))) 
+    (ensures (behavior (Cont (Call cmd arg fnc)) ((convert_call_to_event cmd arg rez) :: t, r))) 
   by (compute ()) = 
   ()
 
 let beh_extend_trace_d
   #a
   (cmd : io_cmds)
-  (argz : io_args cmd)
+  (arg : io_args cmd)
   (rez : io_resm cmd)
-  (fnc : io_resm cmd -> io a)
-  (t:events_trace) :
+  (fnc : maybe (io_res cmd) -> io a)
+  (t:trace) :
   Lemma
     (forall r. (behavior (fnc rez) (t, r) ==>
-      (behavior (Cont (Call cmd argz fnc)) ((convert_call_to_event cmd argz rez) :: t, r)))) =
+      (behavior (Cont (Call cmd arg fnc)) ((convert_call_to_event cmd arg rez) :: t, r)))) =
   Classical.forall_intro (
-    Classical.move_requires (beh_extend_trace cmd argz rez fnc t))
+    Classical.move_requires (beh_extend_trace cmd arg rez fnc t))
 
 let beh_extend_trace_in_bind 
   #a #b
   (cmd : io_cmds)
-  (argz : io_args cmd)
+  (arg : io_args cmd)
   (rez : io_resm cmd)
-  (fnc : io_resm cmd -> io a)
+  (fnc : maybe (io_res cmd) -> io a)
   (k : a -> io b)
-  (t:events_trace)
+  (t:trace)
   (r:maybe b) :
   Lemma
     (requires (behavior (io_bind a b (fnc rez) k) (t, r))) 
-    (ensures (behavior (io_bind a b (Cont (Call cmd argz fnc)) k) ((convert_call_to_event cmd argz rez) :: t, r))) =
+    (ensures (behavior (io_bind a b (Cont (Call cmd arg fnc)) k) ((convert_call_to_event cmd arg rez) :: t, r))) =
   calc (==) {
-    io_bind a b (Cont (Call cmd argz fnc)) k;
+    io_bind a b (Cont (Call cmd arg fnc)) k;
     == {}
-    sys_bind io_cmds io_sig a b (Cont (Call cmd argz fnc)) k;
+    sys_bind io_cmds io_sig a b (Cont (Call cmd arg fnc)) k;
     == { _ by (norm [iota; delta]; compute ()) }
-    Cont (sysf_fmap (Call cmd argz fnc) 
+    Cont (sysf_fmap (Call cmd arg fnc) 
       (fun fnci -> sys_bind io_cmds io_sig a b fnci k));
     == { _ by (norm [delta_only [`%sysf_fmap]]; 
                norm [iota]; 
-               norm [delta_only [`%io_bind]]) }
-    Cont (Call cmd argz (fun rez -> 
+               norm [delta_only [`%io_bind]];
+               compute ()) }
+    Cont (Call cmd arg (fun rez -> 
       io_bind a b (fnc rez) k));
   };
-  beh_extend_trace cmd argz rez (fun rez -> io_bind a b (fnc rez) k) t r;
-  assert (behavior (Cont (Call cmd argz (fun rez -> 
-    io_bind a b (fnc rez) k))) ((convert_call_to_event cmd argz rez) :: t, r)) by (
+  beh_extend_trace cmd arg rez (fun rez -> io_bind a b (fnc rez) k) t r;
+  assert (behavior (Cont (Call cmd arg (fun rez -> 
+    io_bind a b (fnc rez) k))) ((convert_call_to_event cmd arg rez) :: t, r)) by (
     unfold_def (`convert_call_to_event); assumption ())
 
-let extract_result (cmd:io_cmds) (event:io_event) : 
+let extract_result (cmd:io_cmds) (e:event) : 
   Pure (resm cmd)
-    (requires ((cmd == Openfile /\ EOpenfile? event) \/
-               (cmd == Read /\ ERead? event) \/
-               (cmd == Close /\ EClose? event)))
+    (requires ((cmd == Openfile /\ EOpenfile? e) \/
+               (cmd == Read /\ ERead? e) \/
+               (cmd == Close /\ EClose? e)))
     (ensures (fun r -> True)) = 
   match cmd with 
-  | Openfile -> EOpenfile?.r event 
-  | Read -> ERead?.r event 
-  | Close -> EClose?.r event 
+  | Openfile -> EOpenfile?.r e
+  | Read -> ERead?.r e
+  | Close -> EClose?.r e
     
 let rec beh_bind_inl
   #a #b
   (m : io a)
   (k : a -> io b) 
   (r1:a) 
-  (t1 t2 : events_trace)
+  (t1 t2 : trace)
   (r2:maybe b) :
   Lemma 
     (requires (behavior m (t1, (Inl r1)) /\ behavior (k r1) (t2, r2)))
@@ -136,13 +137,13 @@ let rec beh_bind_inl
   match m with
   | Return x -> ()
   | Throw err -> ()
-  | Cont (Call cmd argz fnc) -> begin
+  | Cont (Call cmd arg fnc) -> begin
     let (ht1 :: tt1) = t1 in
     let rez : resm cmd = extract_result cmd ht1 in
     FStar.WellFounded.axiom1 fnc rez;
-    beh_shift_trace cmd argz rez fnc tt1 (Inl r1);
+    beh_shift_trace cmd arg rez fnc tt1 (Inl r1);
     beh_bind_inl (fnc rez) k r1 tt1 t2 r2;
-    beh_extend_trace_in_bind cmd argz rez fnc k (tt1@t2) r2
+    beh_extend_trace_in_bind cmd arg rez fnc k (tt1@t2) r2
   end
   
 let rec beh_bind_inr
@@ -150,19 +151,19 @@ let rec beh_bind_inr
   (m : io a)
   (k : a -> io b)
   (r1:exn)
-  (t1 : events_trace) :
+  (t1 : trace) :
   Lemma 
     (requires (behavior m (t1, (Inr r1))))
     (ensures (behavior (io_bind _ _ m k) (t1, (Inr r1)))) =
   match m with
   | Throw err -> ()
-  | Cont (Call cmd argz fnc) -> begin
+  | Cont (Call cmd arg fnc) -> begin
     let (ht1 :: tt1) = t1 in
     let rez : resm cmd = extract_result cmd ht1 in
     FStar.WellFounded.axiom1 fnc rez;
-    beh_shift_trace cmd argz rez fnc tt1 (Inr r1);
+    beh_shift_trace cmd arg rez fnc tt1 (Inr r1);
     beh_bind_inr (fnc rez) k r1 tt1;
-    beh_extend_trace_in_bind cmd argz rez fnc k (tt1) (Inr r1)
+    beh_extend_trace_in_bind cmd arg rez fnc k (tt1) (Inr r1)
   end
 
 let beh_bind_0 
@@ -203,7 +204,7 @@ let rec beh_bind_tot_0
   (f:io a) 
   (g:a -> Tot b)
   (r1:maybe b)
-  (t:events_trace) :
+  (t:trace) :
   Lemma 
     (requires (behavior (io_bind a b f (fun x -> M4.lift_pure_mfour b (fun p -> p (g x)) (fun _ -> g x) (fun _ -> True))) (t, r1)))
     (ensures (exists r2. inl_app g r2 == r1 /\ behavior f (t, r2)))  =
@@ -214,12 +215,12 @@ let rec beh_bind_tot_0
   | Throw err -> 
       assert (inl_app g (Inr err) == r1);
       assert (behavior f (t, (Inr err)))
-  | Cont (Call cmd argz fnc) ->
+  | Cont (Call cmd arg fnc) ->
     let (ht1 :: tt1) = t in
     let rez : resm cmd = extract_result cmd ht1 in
     FStar.WellFounded.axiom1 fnc rez;
     beh_bind_tot_0 (fnc rez) g r1 tt1;
-    beh_extend_trace_d cmd argz rez fnc (tt1)
+    beh_extend_trace_d cmd arg rez fnc (tt1)
        
 let beh_bind_tot
   #a #b
@@ -239,10 +240,10 @@ let beh_included_bind_tot
       (behavior f)) = 
   beh_bind_tot f g
 
-let beh_iost_to_io (a:Type) (tree:io (events_trace * a)) :
+let beh_iost_to_io (a:Type) (tree:io (trace * a)) :
   Lemma (behavior (IOStHist.iost_to_io tree) `included_in (inl_app cdr)` behavior tree) 
   by (unfold_def (`IOStHist.iost_to_io); norm [iota;delta]; compute ()) =
-  beh_included_bind_tot #(events_trace * a) #a
+  beh_included_bind_tot #(trace * a) #a
     tree
     cdr
 
@@ -275,23 +276,23 @@ let beh_included_in_merge_f_g x y z f g:
 
 let beh_implies_iohist_interp 
   (a : Type)
-  (m : io (events_trace * a)) 
-  (t : events_trace)
-  (r : maybe (events_trace * a)) :
+  (m : io (trace * a)) 
+  (t : trace)
+  (r : maybe (trace * a)) :
   Lemma 
     (requires (behavior m (t,r)))
     (ensures (iohist_interpretation m (fun res le -> (t,res) == (le,r)))) = 
   match m with
   | Return _ -> ()
   | Throw _ -> ()
-  | Cont (Call cmd argz fnc) -> admit ()
+  | Cont (Call cmd arg fnc) -> admit ()
 
 let gio_post_implies_set_of_traces 
   (a : Type)
   (b : Type)
   (pi : monitorable_prop)
-  (t : events_trace)
-  (r : maybe (events_trace * b)) :
+  (t : trace)
+  (r : maybe (trace * b)) :
   Lemma 
     (requires  (m4wp_invariant_post pi [] r t))
     (ensures (pi_to_set pi (t, r))) = 
@@ -301,28 +302,28 @@ let gio_post_implies_set_of_traces
 let iohist_interp_shift_trace
   #a
   (cmd : io_cmds)
-  (argz : args cmd)
+  (arg : args cmd)
   (rez : resm cmd)
   (fnc : resm cmd -> io a)
   p:
   Lemma 
-    (requires (iohist_interpretation (Cont (Call cmd argz fnc)) p))
+    (requires (iohist_interpretation (Cont (Call cmd arg fnc)) p))
     (ensures (
-      iohist_interpretation (fnc rez) (gen_post p (convert_call_to_event cmd argz rez)))) = 
+      iohist_interpretation (fnc rez) (gen_post p (convert_call_to_event cmd arg rez)))) = 
   calc (==) {
-    iohist_interpretation (Cont (Call cmd argz fnc)) p;
+    iohist_interpretation (Cont (Call cmd arg fnc)) p;
     == { _ by (compute ())}
     (forall res. (
-      let event : io_event = convert_call_to_event cmd argz res in
+      let event : io_event = convert_call_to_event cmd arg res in
       iohist_interpretation (fnc res) (gen_post p event)));
   }
 
 let rec gio_interpretation_implies_set_of_traces
   (a : Type)
   (pi : monitorable_prop)
-  (m : io (events_trace * a)) 
-  (le : events_trace)
-  (r : maybe (events_trace * a)) 
+  (m : io (trace * a)) 
+  (le : trace)
+  (r : maybe (trace * a)) 
   p :
   Lemma 
     (requires (iohist_interpretation m p) /\ behavior m (le, r))
@@ -330,13 +331,13 @@ let rec gio_interpretation_implies_set_of_traces
   match m with
   | Return _ -> ()
   | Throw _ -> ()
-  | Cont (Call cmd argz fnc) -> begin
+  | Cont (Call cmd arg fnc) -> begin
     let (ht1 :: tt1) = le in
     let rez : resm cmd = extract_result cmd ht1 in
     FStar.WellFounded.axiom1 fnc rez;
-    beh_shift_trace cmd argz rez fnc tt1 r;
-    iohist_interp_shift_trace cmd argz rez fnc p;
-    gio_interpretation_implies_set_of_traces a pi (fnc rez) tt1 r (gen_post p (convert_call_to_event cmd argz rez))
+    beh_shift_trace cmd arg rez fnc tt1 r;
+    iohist_interp_shift_trace cmd arg rez fnc p;
+    gio_interpretation_implies_set_of_traces a pi (fnc rez) tt1 r (gen_post p (convert_call_to_event cmd arg rez))
   end
 
 
@@ -350,8 +351,8 @@ let beh_gio_implies_post
   (pi : monitorable_prop)
   (ws : a -> M4wp b pi (fun _ _ _ -> True)) 
   (x : a)
-  (t : events_trace)
-  (r : maybe (events_trace * b)) :
+  (t : trace)
+  (r : maybe (trace * b)) :
   Lemma 
     (requires (beh pi ws x (t, r)))
     (ensures  (m4wp_invariant_post pi [] r t)) =
@@ -363,8 +364,8 @@ let beh_gio_in_pi_0
   (pi : monitorable_prop)
   (ws : a -> M4wp b pi (fun _ _ _ -> True)) 
   (x : a)
-  (t : events_trace)
-  (r : maybe (events_trace * b)) :
+  (t : trace)
+  (r : maybe (trace * b)) :
   Lemma 
     (requires ((beh pi ws x) (t, r)))
     (ensures  ((pi_to_set pi) (t, r))) =
