IO.Effect.fst
@@ -98,8 +98,7 @@ layered_effect {
 }
 
 let lift_pure_iowp (a:Type) (wp:pure_wp a) (f:(eqtype_as_type unit -> PURE a wp)) :
-  Pure (io_irepr a (fun s0 p -> wp (fun r -> p (Inl r) []))) (requires True)
-                    (ensures (fun _ -> True))
+  Tot (io_irepr a (fun s0 p -> wp (fun r -> p (Inl r) [])))
   = fun s0 p -> let r = elim_pure f (fun r -> p (Inl r) []) in io_return _ r
 
 sub_effect PURE ~> IOwp = lift_pure_iowp
