Rsp.fst
@@ -1,0 +1,368 @@
+module Rsp
+
+open FStar.Calc
+open FStar.Tactics
+
+open Common
+open ExtraTactics
+
+open IO.Free
+open IO.Effect
+open IIO.Effect
+open MIO.Effect
+open MIIO.Effect
+
+noeq type compiler = {
+  interface : Type;
+  set_of_traces : Type -> Type;
+  monitorable_prop : Type;
+  safety_prop   : (#a:Type) -> monitorable_prop -> set_of_traces a;
+
+  res_s   : interface -> Type;
+  prog_s  : interface -> monitorable_prop -> Type;
+  ctx_s   : interface -> monitorable_prop -> Type;
+  whole_s : interface -> monitorable_prop -> Type;
+  link_s  : (#i:interface) -> (#pi:monitorable_prop) -> ctx_s i pi -> prog_s i pi -> Tot (whole_s i pi);
+
+  res_t   : interface -> Type;
+  prog_t  : interface -> monitorable_prop -> Type;
+  ctx_t   : interface -> Type;
+  whole_t : interface -> Type;
+  link_t  : (#i:interface) -> (#pi:monitorable_prop) -> ctx_t i -> prog_t i pi -> Tot (whole_t i);
+
+
+  beh_s : (#i:interface) -> (#pi:monitorable_prop) -> whole_s i pi -> set_of_traces (res_s i);
+  beh_t : (#i:interface) -> whole_t i -> set_of_traces (res_t i);
+
+  included_in_s : (#i:interface) -> set_of_traces (res_s i) -> set_of_traces (res_s i) -> Type;
+  included_in_t : (#i:interface) -> set_of_traces (res_t i) -> set_of_traces (res_s i) -> Type;
+
+  compile_prog  : (#i:interface) -> (#pi:monitorable_prop) -> prog_s i pi -> Tot (prog_t i pi);
+  compile_whole : (#i:interface) -> (#pi:monitorable_prop) -> whole_s i pi -> Tot (whole_t i);
+}
+  
+noeq type interface = {
+  a : Type; // ad : exportable a;
+  ad : Type;
+  b : Type; // bd : ml b;         // b has to be importable and exportable
+  c : Type; // cd : exportable c;
+  cd : Type;
+  post : a -> trace -> maybe b -> trace -> Type; 
+  //cpost : checkable4 post;
+}
+
+let safety_prop = (#a:Type) -> a -> Type0
+// let safety_prop = pi_to_set
+
+type whole_s (i:interface) (pi:monitorable_prop) = unit -> IIO i.c pi (fun _ _ _ -> True)
+type whole_t (i:interface) = unit -> MIIO i.cd
+
+type ctx_s (i:interface) (pi:monitorable_prop) = (x:i.a) -> IIO i.b pi (i.post x)
+type ctx_p (i:interface) (pi:monitorable_prop) = i.ad -> IIO i.b pi (fun _ _ _ -> True)
+type ctx_t (i:interface) = i.ad -> MIO i.b
+
+type prog_s (i:interface) (pi:monitorable_prop) = ctx_s i pi -> IIO i.c pi (fun _ _ _ -> True)
+type prog_t (i:interface) (pi:monitorable_prop) = ctx_p i pi -> MIIO i.cd
+
+
+let rev_append_rev_append () : Lemma (
+  forall (s0 le1 le2:trace). ((List.rev le2) @ (List.rev le1) @ s0) ==
+     ((List.rev (le1@le2)) @ s0)) =
+  let aux (s0 le1 le2:trace) : Lemma (
+    ((List.rev le2) @ (List.rev le1) @ s0) ==
+       ((List.rev (le1@le2)) @ s0)) = begin
+    List.rev_append le1 le2;
+    List.append_assoc (List.rev le2) (List.rev le1) s0
+  end in Classical.forall_intro_3 aux
+
+
+let rec handle #t2 (tree : iio (t2)) (pi:monitorable_prop) : IIO t2 pi (fun _ _ _ -> True) = begin
+  match tree with
+  | Return r -> r 
+  | Throw r -> IIO.Effect.throw r
+  | Cont (Call GetTrace argz fnc) ->
+      let h = IIO.Effect.get_trace () in
+      FStar.WellFounded.axiom1 fnc (Inl h);
+      let z' = fnc (Inl h) in
+      handle z' pi
+  | Cont (Call cmd argz fnc) ->
+      let rez : res cmd = IIO.Effect.dynamic_cmd cmd pi argz in
+      FStar.WellFounded.axiom1 fnc (Inl rez);
+      let z' : sys cmds all_sig t2 = fnc (Inl rez) in
+      rev_append_rev_append ();
+      handle z' pi
+end
+  
+let import_mio
+  (a b : Type)
+  (pi : monitorable_prop)
+  (f : a -> MIO b) :
+  Tot (a -> IIO b pi (fun _ _ _ -> True)) =
+    fun (x:a) -> 
+        let h = get_trace () in
+        // Cezar: I don't think this is ok.
+        handle (cast_io_iio (reify (f x) h (fun _ _ -> True))) pi
+
+
+let ctx_t_to_ctx_p
+  (i  : interface)
+  (pi : monitorable_prop)
+  (ct : ctx_t i) :
+  Tot (ctx_p i pi) =
+  fun (x:i.ad) -> 
+    let h = get_trace () in
+    // Cezar: I don't think post unfolded like that is ok.
+    handle (cast_io_iio (reify (ct x) h (fun _ _ -> True))) pi
+
+let extract_local_events (s0 s1:trace) :
+  Pure trace
+    (requires (exists le. s1 == apply_changes s0 le))
+    (ensures (fun le -> s1 == apply_changes s0 le)) = 
+  admit ();
+  assert (List.length s1 >= List.length s0);
+  let n : nat = (List.length s1) - (List.length s0) in
+  let (le, _) = List.Tot.Base.splitAt n s1 in
+  List.rev le
+
+let ctx_p_to_ctx_s
+  (i  : interface)
+  (pi : monitorable_prop)
+  (cp  : ctx_p i pi) : 
+  Tot (ctx_s i pi) by (
+    explode ();
+    smt ();
+    let zz = get_binder 9 in 
+    focus (fun () ->
+      let _ = t_destruct zz in
+      iterAll (fun () ->
+        let bs = repeat intro in
+        let b = last bs in (* this one is the equality *)
+        rewrite_eqs_from_context ();
+        norm [iota];
+        ())
+    );
+    let aq = get_binder 12 in
+    focus (fun () -> 
+      let _ = t_destruct aq in
+      let bs1 = intro () in
+      let br = intro () in
+      let b = intro () in (* this one is the equality *)
+      rewrite_eqs_from_context ();
+      // l_to_r [`b];
+      norm [iota];
+      ()
+    );
+    explode ();
+    tadmit ();
+    tadmit ();
+    dump "h"
+  ) =
+  fun (x:i.a) -> 
+    assume (forall x err s0 le. i.post x s0 (Inr err) le == true);
+    let s0 : trace = IIO.Effect.get_trace () in
+    let result : i.b = cp (export x) in
+    let s1 : trace = IIO.Effect.get_trace () in
+    let le = extract_local_events s0 s1 in
+
+    if check4 #i.a #i.b #i.post #i.cpost x s0 (Inl (s1, result)) le then (
+      assert (i.post x s0 (Inl (s1, result)) le);
+      result
+    ) else IOStHist.throw Contract_failure
+
+unfold 
+let beh_s 
+  #a
+  #b
+  (pi:monitorable_prop) 
+  (ws:(x:a -> M4wp b pi (fun _ _ _ -> True))) 
+  (x:a) =
+  behavior (reify (ws x) (m4wp_invariant_post pi []) [])
+
+unfold
+let beh_t #a #b (wt:a -> M4 b) (x:a) =
+  behavior (reify (wt x) (fun _ -> True))
+
+let compile_prog
+  (#i  : interface)
+  (#pi : monitorable_prop)
+  (f  : prog_s i pi) : 
+  Tot (prog_t i pi) =
+    (fun (ct:ctx_p i pi) ->
+      let cs = ctx_p_to_ctx_s i pi ct in
+      let tree : io (trace * i.c) = reify (f cs) (m4wp_invariant_post pi []) [] in
+      export (M4?.reflect (fun _ -> iost_to_io tree) <: MFOUR i.c (fun p -> forall res. p res)))
+
+let compile_whole 
+  (#i  : interface)
+  (#pi : monitorable_prop)
+  (f  : whole_s i pi) : 
+  Tot (whole_t i) =
+    (fun _ ->
+      let tree : io (trace * i.c) = reify (f ()) (m4wp_invariant_post pi []) [] in
+      export (M4?.reflect (fun _ -> iost_to_io tree) <: MFOUR i.c (fun p -> forall res. p res)))
+ 
+val link_s  : (#i:interface) -> (#pi:monitorable_prop) -> ctx_s i pi -> prog_s i pi -> Tot (whole_s i pi)
+let link_s = (fun #i #pi c p -> (fun _ -> p c))
+
+val link_t  : (#i:interface) -> (#pi:monitorable_prop) -> ctx_t i -> prog_t i pi -> Tot (whole_t i)
+let link_t #i #pi c p : whole_t i = (fun _ -> p (ctx_t_to_ctx_p i pi c))
+  
+let res_s   = (fun i -> maybe (trace * i.c))
+let res_t   = (fun i -> maybe (i.cd.etype))
+  
+val included_in_s : (#i:interface) -> set_of_traces (res_s i) -> set_of_traces (res_s i) -> Type0
+let included_in_s = (fun (#i:interface) -> included_in #(res_s i) #(res_s i) id)
+let included_in_t = (fun (#i:interface) -> included_in #(maybe i.cd.etype) #(maybe (trace * i.c)) (inl_app (compose export cdr)))
+
+let tp (i:interface) (pi:monitorable_prop) (ws:whole_s i pi) : Type0 =
+  ((beh_s pi ws () `included_in_s` (safety_prop pi)) ==>  
+    (beh_t (compile_whole ws) () `included_in_t` (safety_prop pi)))
+  
+let seci_respects_tp
+  (i  : interface)
+  (pi : monitorable_prop) 
+  (ws  : whole_s i pi) :
+  Lemma (tp i pi ws) = 
+
+  let wt : whole_t i = compile_whole ws in
+  let included_in_id #a = included_in #a #a (id #a) in
+  let l1 = reify (wt ()) (fun _ -> True) in
+
+  let l2 = reify (
+          (export (M4?.reflect (ref (iost_to_io (reify (ws ()) (m4wp_invariant_post pi []) []))) <: MFOUR i.c (fun p -> forall res. p res)) <: i.cd.etype)) (fun _ -> True) in 
+
+  let l3s = reify (M4?.reflect (ref (iost_to_io (reify (ws ()) (m4wp_invariant_post pi []) []))) <: MFOUR i.c (fun p -> forall res. p res)) in
+  // TODO: Cezar: is the 3rd argument correct? I suppose it should use pre and post
+  // behavior (M4.ibind i.c i.cd.etype (fun p -> forall res. p res) (fun x -> m4_return_wp (i.cd.etype) (export x))
+  let l3 = (M4.ibind i.c i.cd.etype (fun p -> forall res. p res) (fun x -> m4_return_wp (i.cd.etype) (export x))
+          (l3s)
+          (fun x -> lift_pure_mfour i.cd.etype (fun p -> p (export x)) (fun _ -> export x)) (fun _ -> True)) in
+
+  assert (l1 == l2) by (norm [delta_only [`%compile_whole]]);
+  assert (behavior l1 `included_in id` behavior l2);
+  // TODO: Cezar: this should be just an unfolding of `reify`. I talked with Guido
+  // and it seems using tactics is not a solution to unfold `reify` for 
+  // layered effects because: "reification of layered effects is explicitly disabled
+  // since it requires producing the indices for the bind, and we do not store them
+  // anywhere". I tried to manually unfold looking at EMF* (Dijkstra Monads for
+  // Free), but it seems that F* does not accept this proof. I created a new file only
+  // for this problem: `UnfoldReify.fst`.
+  // Related github issue: https://github.com/FStarLang/FStar/issues/2163
+  assume (behavior l2 `included_in id` behavior l3);
+
+  beh_included_bind_tot #i.c #i.cd.etype
+      (l3s (compute_post i.c (Mkexportable?.etype i.cd) (fun x -> m4_return_wp (Mkexportable?.etype i.cd) (export x)) (fun _ -> True)))
+      export;
+
+  assert (
+      behavior l3
+      `included_in (inl_app export)`
+      behavior (l3s (fun _ -> True))
+  ) by (norm [delta_only [`%ibind]]);
+
+  assert (
+      behavior (l3s (fun _ -> True))
+      `included_in id`
+      behavior (iost_to_io (reify (ws ()) (m4wp_invariant_post pi []) []))
+  );
+
+  beh_iost_to_io i.c (reify (ws ()) (m4wp_invariant_post pi []) []);
+
+  assert (
+      behavior (iost_to_io (reify (ws ()) (m4wp_invariant_post pi []) []))
+      `included_in (inl_app cdr)` 
+      beh_s pi ws ())
+
+val import_ctx_t : (#i:interface) -> (#pi:monitorable_prop) -> ctx_t i -> ctx_s i pi
+let import_ctx_t #i #pi ct =
+  ctx_p_to_ctx_s i pi (
+    ctx_t_to_ctx_p i pi ct)
+
+let beh_export_ps_ct_in_export_ws
+  (i  : interface)
+  (pi : monitorable_prop)
+  (ps : prog_s i pi)
+  (ct : ctx_t i) : 
+  Lemma (
+    let (cs : ctx_s i pi) = import_ctx_t #i #pi ct in
+    let ws : whole_s i pi = cs `link_s #i` ps in
+    let pt : prog_t i pi = compile_prog ps in
+    let wt : whole_t i = compile_whole #i #pi ws in
+    beh_t (ct `link_t` pt) () `included_in id` beh_t wt ()
+  ) = 
+  let cp = ctx_t_to_ctx_p i pi ct in
+  let (cs : ctx_s i pi) = ctx_p_to_ctx_s i pi cp in
+  let ws : whole_s i pi = cs `link_s` ps in
+  let (cs : ctx_s i pi) = ctx_p_to_ctx_s i pi cp in
+  let pt : prog_t i pi = compile_prog ps in
+  let wt : whole_t i = compile_whole ws in
+  assert (reify (pt cp) (fun _ -> True) == reify (wt ()) (fun _ -> True)) by (
+    norm [delta_only [`%compile_prog]];
+    norm [delta_only [`%compile_whole]];
+    norm [delta_only [`%link_s]]
+  );
+  assert (
+    beh_t (ct `link_t #i #pi` pt) ()
+      `included_in id`
+    beh_t ((fun _ -> pt cp) <: whole_t i) ()) 
+  by (norm [delta_only [`%link_t]])
+
+let seci_rsp_0
+  (i   : interface)
+  (pi  : monitorable_prop)
+  (ps  : prog_s i pi)
+  (ct  : ctx_t i) :
+  Lemma (
+  (forall (cs:ctx_s i pi). 
+    (beh_s pi (cs `link_s` ps) ()) `included_in_s` (safety_prop pi))
+  ==>  (
+      let pt = compile_prog #i ps in
+      beh_t (ct `link_t #i #pi` pt) () `included_in_t` (safety_prop pi))) =
+  let (cp:ctx_p i pi) = ctx_t_to_ctx_p i pi ct in
+  let (cs:ctx_s i pi) = ctx_p_to_ctx_s i pi cp in
+  let ws : whole_s i pi = link_s cs ps in
+  beh_gio_in_pi _ _ pi ws (); // Beh (ws ()) in pi
+  seci_respects_tp i pi ws; // Beh (export ws ()) in Beh (ws ())
+  beh_export_ps_ct_in_export_ws i pi ps ct // Beh ((export ps) ct) in Beh (export ws ())
+
+let rsp (i:interface) (pi:monitorable_prop) (ps:prog_s i pi) : Type0 =
+  (forall cs. beh_s pi (cs `link_s` ps) () `included_in_s` (safety_prop (pi)))
+  ==> (forall (ct: ctx_t i). (
+      let pt = compile_prog ps in
+      beh_t (ct `link_t` pt) () `included_in_t` (safety_prop (pi))))
+
+let seci_respects_rsp () :
+  Lemma (forall i pi ps. rsp i pi ps) =
+    Classical.forall_intro_4 (seci_rsp_0)
+  
+
+
+// let seci : compiler = {
+//   interface = interface;
+//   monitorable_prop = monitorable_prop;
+//   safety_prop = pi_to_set;
+
+//   set_of_traces = set_of_traces;
+
+//   res_s   = (fun i -> maybe (trace * i.c));
+//   prog_s  = prog_s;
+//   ctx_s   = ctx_s;
+//   whole_s = whole_s;
+  
+//   link_s = link_s;
+
+//   res_t   = (fun i -> maybe (i.cd.etype));
+//   prog_t  = prog_t;
+//   ctx_t   = ctx_t;
+//   whole_t = whole_t;
+//   link_t = link_t;
+
+//   beh_s = (fun #i #pi w -> beh_s #unit #i.c pi w ());
+//   beh_t = (fun #i w -> beh_t #unit #i.cd.etype w ());
+  
+//   included_in_s = included_in_s;
+//   included_in_t = included_in_t;
+
+//   compile_prog  = compile_prog;
+//   compile_whole = compile_whole;
+// }
