Test.Webserver.fst
@@ -1,0 +1,158 @@
+module Test.Webserver
+
+open Common
+open IO.Free
+open IO.Effect
+open IIO.Effect
+open MIO.Effect
+open MIIO.Effect
+open FStar.All
+open FStar.Tactics
+open ExtraTactics
+
+
+// Case 1. Verified web server tries to enforce pi on
+//         plugin 
+
+val allowed_file : string -> bool
+let allowed_file fnm = match fnm with
+  | "../Makefile" -> false
+  | "Demos.fst" -> true
+  | _ -> false
+
+val allowed_fd : file_descr -> trace -> bool
+let rec allowed_fd fd s0 =
+  match s0 with
+  | [] -> false
+  | EOpenfile fnm (Inl fd') :: t -> if fd = fd' then allowed_file(fnm)
+                                  else allowed_fd fd t
+  | EClose fd' _  :: t -> if fd = fd' then false else allowed_fd fd t
+  | _ :: t -> allowed_fd fd t
+
+let pi : monitorable_prop = (fun s0 action -> 
+  match action with
+  | (| Openfile, fnm |) -> allowed_file(fnm)
+  | (| Read, fd |) -> allowed_fd fd s0
+  | (| Close, fd |) -> allowed_fd fd s0)
+
+// the plugin will be written in GIO (should be ML?)
+// let plugin_type = (pi:monitorable_prop) -> file_descr -> IIO file_descr pi (fun _ r le -> Inl? r /\ is_open (Inl?.v r) le)
+let plugin_type = file_descr -> IIO file_descr pi (fun _ _ _ -> True)
+let ml_plugin_type = file_descr -> MIO file_descr 
+
+// ex1. the webserver register a log for every run of a plugin
+// ex2. given an URL, plugin only opens that URL
+// ex3. The plugin will pass a file_Descr back to the webserver. What can the webserver assume?
+// ex4. Pass a proof to the plugin that a file_descr is open.
+
+let rev_append_rev_append () : Lemma (
+  forall (s0 le1 le2:trace). ((List.rev le2) @ (List.rev le1) @ s0) ==
+     ((List.rev (le1@le2)) @ s0)) =
+
+
+  let aux (s0 le1 le2:trace) : Lemma (
+    ((List.rev le2) @ (List.rev le1) @ s0) ==
+       ((List.rev (le1@le2)) @ s0)) = begin
+    List.rev_append le1 le2;
+    List.append_assoc (List.rev le2) (List.rev le1) s0
+  end in Classical.forall_intro_3 aux
+
+// import plugin_type 
+let webserver (plugin:plugin_type) : IIO unit pi (fun _ _ _ ->True) =
+  rev_append_rev_append ();
+  let fd = pi_static_cmd Openfile pi "Demos.fst" in
+  let _ = plugin fd in
+  ()
+
+let ml_plugin1 : ml_plugin_type = fun fd ->
+  unsafe_cmd Close fd;
+  fd
+  
+let ml_plugin2 : ml_plugin_type = fun fd ->
+  let d = unsafe_cmd Read fd in
+  fd
+
+let ml_plugin3 : ml_plugin_type = fun fd ->
+  let fd = unsafe_cmd Openfile "Demos.fst" in
+  let d = unsafe_cmd Read fd in
+  fd
+
+
+
+let rec handle #t2 (tree : iio (t2)) (pi:monitorable_prop) : IIO t2 pi (fun _ _ _ -> True) = begin
+  match tree with
+  | Return r -> r 
+  | Throw r -> throw r
+  | Cont (Call GetTrace argz fnc) ->
+      let h = get_trace () in
+      FStar.WellFounded.axiom1 fnc (Inl h);
+      let z' = fnc (Inl h) in
+      handle z' pi
+  | Cont (Call cmd argz fnc) ->
+      let rez : res cmd = dynamic_cmd cmd pi argz in
+      FStar.WellFounded.axiom1 fnc (Inl rez);
+      let z' : sys cmds all_sig t2 = fnc (Inl rez) in
+      rev_append_rev_append ();
+      handle z' pi
+end
+  
+let import_mio
+  (a b : Type)
+  (pi : monitorable_prop)
+  (f : a -> MIO b) :
+  Tot (a -> IIO b pi (fun _ _ _ -> True)) =
+    fun (x:a) -> 
+        let h = get_trace () in
+        // Cezar: I don't think this is ok.
+        handle (cast_io_iio (reify (f x) h (fun _ _ -> True))) pi
+
+let plugin1 = import_mio _ _ pi ml_plugin1
+let plugin2 = import_mio _ _ pi ml_plugin2
+let plugin3 = import_mio _ _ pi ml_plugin3
+
+let whole1 () : IIO unit pi (fun _ _ _ -> True) = webserver plugin1
+let whole2 () : IIO unit pi (fun _ _ _ -> True) = webserver plugin2
+let whole3 () : IIO unit pi (fun _ _ _ -> True) = webserver plugin3
+
+// let _ = 
+//   try_with
+//     (fun _ -> webserver' (plugin1))
+//     (fun (err:exn) -> 
+//       match err with
+//       | Contract_failure -> 
+//           FStar.IO.print_any "plugin1 failed successfully\n\n" 
+//       | err -> raise err)
+
+// let _ = 
+//   try_with
+//     (fun _ -> webserver' (plugin2))
+//     (fun (err:exn) -> 
+//       match err with
+//       | Contract_failure -> 
+//           FStar.IO.print_any "plugin2 failed successfully\n\n" 
+//       | err -> raise err)
+
+
+// let _ = 
+//   try_with
+//     (fun _ -> webserver' (plugin3);
+//       FStar.IO.print_any "plugin3 executed successfully\n\n" )
+//     (fun (err:exn) -> raise err)
+
+
+
+
+
+
+
+
+
+
+
+
+// Case 2. Verified code wants to interact with a
+//         verified library and wants to enforce extra pi
+
+
+// Case 3. ML code wants to interact with verifed code and 
+//         and wants to enforce extra pi. (similar with middleware?)
